Cleanup of Memo

examples/dm4free/FStar.DM4F.Memo.fst
@@ -1,5 +1,8 @@
 module FStar.DM4F.Memo
 
+open FStar.Classical
+open FStar.Squash
+
 (* These should be indices of our effect *)
 type dom : eqtype = int
 type codom : Type = int
@@ -26,6 +29,18 @@ new_effect_for_free {
     ; put = put
 }
 
+(* Specification-less version of the memoization effect *)
+effect Memo (a:Type) = MEMO a (fun _ p -> forall z. p z)
+
+(* Access to the whole heap (for verification-debugging purpose) *)
+private
+let get_heap () : MEMO heap (fun h0 p -> p (h0, h0))
+= let f : MEMO?.repr heap (fun h0 p -> p (h0, h0)) = fun h0 -> h0, h0 in
+  MEMO?.reflect f
+
+
+(* Lemmas about lists *)
+
 let rec for_all_prop (#a:Type) (p:a -> Type0) (l:list a) : Tot Type0 (decreases l)
 = match l with
   | [] -> True
@@ -38,24 +53,6 @@ let rec for_all_prop_assoc_lemma (#a:eqtype) (#b:Type) (x:a) (p : (a * b) -> Tot
   | [] -> ()
   | (x0, y0) :: xs -> if x0 = x then () else for_all_prop_assoc_lemma x p xs
 
-
-let valid_memo (h:heap) (f:dom -> Tot codom) = for_all_prop (fun (x,y) -> y == f x) h
-let valid_memo_preserve (x:dom) (y:codom) (h:heap) (f:dom -> Tot codom)
-  : Lemma (requires (y == f x /\ valid_memo h f)) (ensures (valid_memo ((x,y)::h) f))
-= ()
-
-private
-let get_heap () : MEMO heap (fun h0 p -> p (h0, h0))
-= let f : MEMO?.repr heap (fun h0 p -> p (h0, h0)) = fun h0 -> h0, h0 in
-  MEMO?.reflect f
-
-(* let my_put (x:dom) (y:codom) (f:dom -> Tot codom) : MEMO unit (fun h0 p -> valid_memo h0 f /\ y == f x /\ (valid_memo ((x,y)::h0) f ==> p ((), (x,y)::h0))) *)
-(* = let f : MEMO?.repr unit (fun h0 p -> valid_memo h0 f /\ y == f x /\ (valid_memo ((x,y)::h0) f ==> p ((), (x,y)::h0))) = *)
-(*     fun h0 -> ((), (x,y)::h0) *)
-(*   in *)
-(*   MEMO?.reflect f *)
-
-
 let forall_prop_assoc_lemma2 (#a:eqtype) (#b:Type) (x:a) (y:b) (p : (a * b) -> Tot Type0)
   : Lemma (forall h. for_all_prop p h /\ List.assoc x h == Some y ==> p (x,y))
 = let aux h : Lemma (requires (for_all_prop p h /\ List.assoc x h == Some y)) (ensures (p (x,y))) =
@@ -63,7 +60,21 @@ let forall_prop_assoc_lemma2 (#a:eqtype) (#b:Type) (x:a) (y:b) (p : (a * b) -> T
   in
   FStar.Classical.(forall_intro (move_requires aux))
 
-let memo_f (f : dom -> Tot codom) (x:dom) : MEMO codom (fun h0 p -> valid_memo h0 f /\ (forall h. valid_memo h f ==> p (f x, h)))
+let valid_memo (h:heap) (f:dom -> Tot codom) = for_all_prop (fun (x,y) -> y == f x) h
+let valid_memo_preserve (x:dom) (y:codom) (h:heap) (f:dom -> Tot codom)
+  : Lemma (requires (y == f x /\ valid_memo h f)) (ensures (valid_memo ((x,y)::h) f))
+= ()
+
+(* [f `computes` g] when the memoized function [f] computes the same total/pure *)
+(* function as [g] provided the heap contains only [g]-relevant elements *)
+let computes (#p:dom -> Tot Type0) ($f: x:dom{p x} -> Memo codom) (g:dom -> Tot codom) =
+      forall h0. valid_memo h0 g ==> (forall x. p x ==> (let y ,h1 = reify (f x) h0 in y == g x /\ valid_memo h1 g))
+
+
+
+(* Memoization of a pure function with a complete specification *)
+
+let memo_ (f : dom -> Tot codom) (x:dom) : MEMO codom (fun h0 p -> valid_memo h0 f /\ (forall h. valid_memo h f ==> p (f x, h)))
 = match MEMO?.get x with
   | Some y ->
     forall_prop_assoc_lemma2 x y (fun (x,y) -> y == f x) ;
@@ -73,8 +84,11 @@ let memo_f (f : dom -> Tot codom) (x:dom) : MEMO codom (fun h0 p -> valid_memo h
     MEMO?.put x y ;
     y
 
+
+(* Specification-less memoization of a pure function and its extrinsic proof *)
+
 reifiable
-let memo_f_extr (f : dom -> Tot codom) (x:dom) : MEMO codom (fun h0 p -> (forall z. p z))
+let memo_extr (f : dom -> Tot codom) (x:dom) : Memo codom
 = match MEMO?.get x with
   | Some y -> y
   | None ->
@@ -82,26 +96,28 @@ let memo_f_extr (f : dom -> Tot codom) (x:dom) : MEMO codom (fun h0 p -> (forall
     MEMO?.put x y ;
     y
 
-
-let memo_f_extr_lemma (f:dom -> Tot codom) (x:dom) (h0:heap)
+let memo_extr_lemma (f:dom -> Tot codom) (x:dom) (h0:heap)
   : Lemma (requires (valid_memo h0 f))
-    (ensures (let (y, h1) = reify (memo_f_extr f x) h0 in valid_memo h1 f /\ y == f x))
+    (ensures (let (y, h1) = reify (memo_extr f x) h0 in valid_memo h1 f /\ y == f x))
 = match reify (MEMO?.get x) h0 with
-  | Some y, h0' ->
-    forall_prop_assoc_lemma2 x y (fun (x,y) -> y == f x)
-  | None, h0' ->
-    ()
+  | Some y, h0' -> forall_prop_assoc_lemma2 x y (fun (x,y) -> y == f x)
+  | None, h0' -> ()
+
+let memo_extr_computes (f:dom -> Tot codom) : Lemma ((memo_extr f) `computes` f) =
+  let phi0 (h0:heap) (vm:squash(valid_memo h0 f)) (x:dom)
+    : Lemma (let y, h1 = reify (memo_extr f x) h0 in y == f x /\ valid_memo h1 f) =
+    give_proof vm ; memo_extr_lemma f x h0
+  in
+  forall_impl_intro (fun (h0:heap) (vm:squash(valid_memo h0 f)) -> forall_intro (phi0 h0 vm) <:
+    Lemma (forall x. let y, h1 = reify (memo_extr f x) h0 in y == f x /\ valid_memo h1 f))
 
 
 
 
-effect Memo (a:Type) = MEMO a (fun _ p -> forall z. p z)
-
-let computes (#p:dom -> Tot Type0) ($f: x:dom{p x} -> Memo codom) (g:dom -> Tot codom) =
-  forall h0. valid_memo h0 g ==> (forall x. p x ==> (let y ,h1 = reify (f x) h0 in y == g x /\ valid_memo h1 g))
+(* Specification-less memoization of a memoized function and its extrinsic proof *)
 
 reifiable
-let memo_f_extr_p (p:dom -> Type0) (f : x:dom{p x} -> Memo codom) (x:dom{p x}) : Memo codom
+let memo_extr_p (p:dom -> Type0) (f : x:dom{p x} -> Memo codom) (x:dom{p x}) : Memo codom
 = match MEMO?.get x with
   | Some y -> y
   | None ->
@@ -109,15 +125,9 @@ let memo_f_extr_p (p:dom -> Type0) (f : x:dom{p x} -> Memo codom) (x:dom{p x}) :
     MEMO?.put x y ;
     y
 
-(* let valid_memo_p (h:heap) (p:dom -> Type0) (f: x:dom{p x} -> Memo codom) = for_all_prop (fun (x,y) -> p x ==> y == fst (reify (f x) h)) h *)
-(* let valid_memo_preserve (x:dom) (y:codom) (h:heap) (f:dom -> Tot codom) *)
-(*   : Lemma (requires (y == f x /\ valid_memo h f)) (ensures (valid_memo ((x,y)::h) f)) *)
-(*   = () *)
-
-
-let memo_f_extr_p_lemma (p:dom -> Type0) (f: x:dom{p x} -> Memo codom) (g:dom -> Tot codom) (h0:heap) (x:dom)
+let memo_extr_p_lemma (p:dom -> Type0) (f: x:dom{p x} -> Memo codom) (g:dom -> Tot codom) (h0:heap) (x:dom)
   : Lemma (requires (valid_memo h0 g /\ f `computes` g))
-    (ensures (p x ==> (let (y, h1) = reify (memo_f_extr_p p f x) h0 in y == g x /\ valid_memo h1 g)))
+    (ensures (p x ==> (let (y, h1) = reify (memo_extr_p p f x) h0 in y == g x /\ valid_memo h1 g)))
 = match reify (MEMO?.get x) h0 with
   | Some y, h0' ->
     forall_prop_assoc_lemma2 x y (fun (x,y) -> y == g x)
@@ -125,66 +135,83 @@ let memo_f_extr_p_lemma (p:dom -> Type0) (f: x:dom{p x} -> Memo codom) (g:dom ->
     ()
 
 
-
-let memo_f_extr_computes (p:dom -> Type0) (f: x:dom{p x} -> Memo codom) (g:dom -> Tot codom)
-: Lemma (requires (f `computes` g)) (ensures ((memo_f_extr_p p f) `computes` g))
+(* If [f `computes` g] then the memoized version of [f], [memo_extr_p p f] also computes [g] *)
+let memo_extr_p_computes (p:dom -> Type0) (f: x:dom{p x} -> Memo codom) (g:dom -> Tot codom)
+: Lemma (requires (f `computes` g)) (ensures ((memo_extr_p p f) `computes` g))
 =
   let open FStar.Squash in
   let phi0 (fcg:squash(f `computes` g)) (h0:heap) (vm : squash (valid_memo h0 g)) (x:dom)
-    : Lemma (p x ==> (let y ,h1 = reify (memo_f_extr_p p f x) h0 in y == g x /\ valid_memo h1 g))
+    : Lemma (p x ==> (let y ,h1 = reify (memo_extr_p p f x) h0 in y == g x /\ valid_memo h1 g))
   = give_proof fcg ;
     give_proof vm ;
-    memo_f_extr_p_lemma p f g h0 x
+    memo_extr_p_lemma p f g h0 x
   in
-  let phi1 (fcg:squash(f `computes` g)) (h0:heap) () : Lemma (requires (valid_memo h0 g)) (ensures (forall x. p x ==> (let (y, h1) = reify (memo_f_extr_p p f x) h0 in y == g x /\ valid_memo h1 g))) =
+  let phi1 (fcg:squash(f `computes` g)) (h0:heap) () : Lemma (requires (valid_memo h0 g)) (ensures (forall x. p x ==> (let (y, h1) = reify (memo_extr_p p f x) h0 in y == g x /\ valid_memo h1 g))) =
     FStar.Classical.forall_intro (phi0 fcg h0 (get_proof (valid_memo h0 g)))
   in
   let phi2 fcg (h0:heap)
-    : Lemma (valid_memo h0 g ==> (forall x. p x ==> (let y ,h1 = reify (memo_f_extr_p p f x) h0 in y == g x /\ valid_memo h1 g)))
+    : Lemma (valid_memo h0 g ==> (forall x. p x ==> (let y ,h1 = reify (memo_extr_p p f x) h0 in y == g x /\ valid_memo h1 g)))
   = FStar.Classical.move_requires (phi1 fcg h0) () in
   FStar.Classical.forall_intro (phi2 (get_proof (f `computes` g)))
 
 
 (* reifiable *)
-(* let memo_f_extr (f : dom -> Tot codom) (x:dom) : MEMO codom (fun h0 p -> (forall z. p z)) *)
-(* = memo_f_extr_p (fun _ -> True) f x *)
+(* let memo_extr (f : dom -> Tot codom) (x:dom) : MEMO codom (fun h0 p -> (forall z. p z)) *)
+(* = memo_extr_p (fun _ -> True) f x *)
 
 (* (\* Should work but does not... *\) *)
 (* (\* needs induction to prove valid_memo h0 f ==> valid_memo_p h0 (fun _ -> True) f ? *\) *)
 
-(* let memo_f_extr_lemma (f:dom -> Tot codom) (x:dom) (h0:heap) *)
+(* let memo_extr_lemma (f:dom -> Tot codom) (x:dom) (h0:heap) *)
 (*     : Lemma (requires (valid_memo h0 f)) *)
-(*       (ensures (let (y, h1) = reify (memo_f_extr f x) h0 in valid_memo h1 f /\ y == f x)) *)
+(*       (ensures (let (y, h1) = reify (memo_extr f x) h0 in valid_memo h1 f /\ y == f x)) *)
 (* = assert (valid_memo_p h0 (fun _ -> True) f) ; *)
-(*   memo_f_extr_p_lemma (fun _ -> True) f x h0 *)
+(*   memo_extr_p_lemma (fun _ -> True) f x h0 *)
 
 
 
+(* Tentaive approach to memoization of recursive functions *)
+(* Given a function [f : x0:dom -> f0:(x:dom{x << x0} -> Tot codom) -> Tot codom] *)
+(* we can compute its fixpoint as follow with [fix f] *)
 
 let fix (f : x0:dom -> f0:(x:dom{x << x0} -> Tot codom) -> Tot codom) (x0:dom) : Tot codom
 = let rec f0 (x:dom{x << x0}) = f x f0 in
   f x0 f0
 
+(* A first idea would be to extend the fixpoint to a memoized fixpoint but this clearly *)
+(* does not work since the [f0] continuation that we would feed to [f] would need *)
+(* to have a [Memo] effect and not a total one. *)
 
-noeq type partial_result : dom -> Type =
-| Done : x0:dom -> codom -> partial_result x0
-| Need : x0:dom -> x:dom{x << x0} -> (codom -> Tot (partial_result x0)) -> partial_result x0
+(* So instead we introduce a notion of partial result which can be : *)
+noeq type partial_result (x0:dom) : Type =
 
+(* Either a terminated computation of type codom *)
+| Done : codom -> partial_result x0
+
+(* Or a computation asking for the result of the recursive call on [x] and a continuation [cont] *)
+| Need : x:dom{x << x0} -> cont:(codom -> Tot (partial_result x0)) -> partial_result x0
+
+
+(* We can define the actual total function represented *)
+(* by [f : x:dom -> Tot (partial_result x)] with *)
+(* [fixp f : dom -> Tot codom] *)
 
 let rec  complete_fixp (f: (x:dom) -> partial_result x) (x:dom) (px:partial_result x) : Tot codom (decreases %[x ; px]) =
   match px with
-  | Done _ y -> y
-  | Need x0 x' cont ->
+  | Done y -> y
+  | Need x' cont ->
     assume (forall y. cont y << cont) ;
     complete_fixp f x (cont (complete_fixp f x' (f x')))
 
 let fixp (f: x:dom -> Tot (partial_result x)) (x0:dom) : Tot codom
   = complete_fixp f x0 (f x0)
 
-noeq type reachable (f: (x:dom) -> partial_result x) x : partial_result x -> Type0 =
-    | Now : reachable f x (f x)
-    | Later : x0:dom{x0 << x} -> cont:(codom -> Tot (partial_result x)) -> reachable f x (Need x x0 cont) -> reachable f x (cont (fixp f x0))
 
+(* Lemmas about partial results *)
+
+noeq type reachable (f: (x0:dom) -> partial_result x0) x0 : partial_result x0 -> Type0 =
+| Now : reachable f x0 (f x0)
+| Later : x:dom{x << x0} -> cont:(codom -> Tot (partial_result x0)) -> reachable f x0 (Need x cont) -> reachable f x0 (cont (fixp f x))
 
 let rec reachable_lemma f x px (w:reachable f x px)
   : Lemma (requires True)
@@ -193,23 +220,28 @@ let rec reachable_lemma f x px (w:reachable f x px)
 = match w with
   | Now -> assert (px == f x) ; assert (complete_fixp f x px == fixp f x)
   | Later x0 cont w' ->
-    reachable_lemma f x (Need x x0 cont) w'
+    reachable_lemma f x (Need x0 cont) w'
+
 
 let rec fpartial_result x (f: (x:dom) -> partial_result x) (px:partial_result x) : Tot Type0 (decreases px) =
   match px with
-  | Done x0 y -> y == fixp f x
-  | Need x0 x1 cont ->
+  | Done y -> y == fixp f x
+  | Need x1 cont ->
     assume (forall y. cont y << cont) ;
     fpartial_result x f (cont (fixp f x1))
 
 
 let rec fpartial_result_lemma f x px (w:reachable f x px) : Lemma (requires True) (ensures (fpartial_result x f px)) (decreases px)
 = match px with
-  | Done _ y -> reachable_lemma f x px w (* ; assert (y == fixp f x) ;     assert (fpartial_result x f px) *)
+  | Done y -> reachable_lemma f x px w (* ; assert (y == fixp f x) ;     assert (fpartial_result x f px) *)
 
-  | Need x1 x' cont -> assume (forall y. cont y << cont) ;
+  | Need x' cont -> assume (forall y. cont y << cont) ;
     let px' = cont (fixp f x') in
     fpartial_result_lemma f x px' (Later x' cont w)
+
+
+
+(* Memoization of a recursive functions represented as [f : x:dom -> partial_result x] with a complete spec *)
 
 let valid_memo_rec (h:heap) (f: x:dom -> Tot (partial_result x)) = for_all_prop (fun (x,y) -> y == fixp f x) h
 
@@ -228,17 +260,14 @@ let valid_memo_rec_lemma
 let rec complete_memo_rec (f: x:dom -> Tot (partial_result x)) (x:dom) (px:partial_result x{fpartial_result x f px})
   : MEMO codom (memo_rec_wp f x) (decreases %[x ; px])
 = match px with
-  | Done _ y -> assert (y == fixp f x) ; y
-  | Need x1 x' cont ->
-    assert (x1 == x) ;
+  | Done y -> assert (y == fixp f x) ; y
+  | Need x' cont ->
     let y : (y:codom{y == fixp f x'}) =
       let h0 = get_heap () in
       assert (valid_memo_rec h0 f) ;
       match MEMO?.get x' with
       | Some y ->
         valid_memo_rec_lemma f x' y h0 ;
-        (* for_all_prop_assoc_lemma x' (fun (x',y) -> y == fixp f x') h0 ; *)
-        (* forall_prop_assoc_lemma2 x' y (fun (x',y) -> y == fixp f x') ; *)
         assert (y == fixp f x') ;
         y
       | None ->
@@ -272,112 +301,98 @@ let memo_rec (f: x:dom -> Tot (partial_result x)) (x0:dom)
 
 
 
-let p (x:dom) (px:partial_result x) (x':dom) = %[ %[x'; 1 ; ()] ] << %[ %[x; 0 ; px] ]
+
+
+(* ****************************************************************************)
+(*                                                                            *)
+(*        Specification-less memoization of recursive function                *)
+(*        and extrinsic proofs (using reification)                            *)
+(*                                                                            *)
+(* ****************************************************************************)
+
+
+let p (x:dom) (px:partial_result x) (x':dom) = %[ %[x'; 2 ; ()] ] << %[ %[x; 0 ; px] ]
 
 reifiable
 let rec complete_memo_rec_extr
   (f: (x:dom) -> partial_result x)
   (x:dom)
   (px:partial_result x)
-  : Memo codom (decreases %[x ; 0 ; px])
+  : Memo codom (decreases %[x ; 1 ; px])
 =
   match px with
-  | Done _ y -> y
-  | Need x0 x' cont ->
-      let y = memo_f_extr_p (p x px) (memo_rec_extr_temp f x px) x' in
+  | Done y -> y
+  | Need x' cont ->
+    let y = memo_extr_p (p x px) (memo_rec_extr_temp f x px) x' in
     assume (forall y. cont y << cont) ;
     complete_memo_rec_extr f x (cont y)
 
 and memo_rec_extr_temp (f: (x:dom) -> partial_result x) (x0:dom) (px0:partial_result x0) (x:dom{p x0 px0 x})
-  : Memo codom
+  : Memo codom (decreases %[x0 ; 0 ; px0])
 = memo_rec_extr f x
 
-and memo_rec_extr (f: x:dom -> Tot (partial_result x)) (x0:dom) : Memo codom (decreases %[ x0 ; 1 ; ()])
+and memo_rec_extr (f: x:dom -> Tot (partial_result x)) (x0:dom) : Memo codom (decreases %[ x0 ; 2 ; ()])
 = complete_memo_rec_extr f x0 (f x0)
 
 
-(* let rec complete_memo_rec_extr_computes *)
-(*   (f: (x:dom) -> partial_result x) *)
-(*   (x:dom) *)
-(*   (px:partial_result x) *)
-(*   (h0:heap) *)
-(*   : Lemma (requires (fpartial_result x f px /\ valid_memo h0 (fixp f) /\ (memo_rec_extr f) `computes` (fixp f))) *)
-(*     (ensures (let y, h1 = reify (complete_memo_rec_extr f x px) h0 in y == fixp f x /\ valid_memo h1 (fixp f))) *)
-(*     (decreases px) *)
-(* = *)
-(*   match px with *)
-(*   | Done _ y -> () *)
-(*   | Need _ x' cont -> *)
-(*     memo_f_extr_computes (fun x' -> %[ %[x'; 1 ; ()] ] << %[ %[x; 0 ; px] ]) (memo_rec_extr f) (fixp f) ; *)
-(*     let y, h1 = reify (memo_f_extr_p (fun x' -> %[ %[x'; 1 ; ()] ] << %[ %[x; 0 ; px] ]) (memo_rec_extr f) x') h0 in *)
-(*     assert (y == fixp f x') ; *)
-(*     assert (valid_memo h1 (fixp f)) ; *)
-(*     assume (forall y. cont y << cont) ; *)
-(*     complete_memo_rec_extr_computes f x (cont y) h1 *)
+let rec complete_memo_rec_extr_computes :
+  (f:(x:dom -> partial_result x)) ->
+  (x:dom) ->
+  (px:partial_result x) ->
+  (h0:heap) ->
+  Lemma (requires (fpartial_result x f px /\ valid_memo h0 (fixp f)))
+    (ensures (let y, h1 = reify (complete_memo_rec_extr f x px) h0 in y == fixp f x /\ valid_memo h1 (fixp f)))
+    (decreases %[x ; 1 ; px])
+= fun f x px h0 ->
+  match px with
+  | Done y -> ()
+  | Need x' cont ->
+    let compute_lemma0 (h0:heap) (vm:squash(valid_memo h0 (fixp f))) (x':dom) (px':squash (p x px x'))
+        : Lemma (p x px x' ==> (let y, h1 = reify (memo_rec_extr_temp f x px x') h0 in
+                               y == fixp f x' /\ valid_memo h1 (fixp f)))
+    = give_proof vm ; give_proof px' ; assert (%[ %[x; 0 ; px] ] << %[ %[x; 1 ; px] ]); memo_rec_extr_computes f x' h0
+    in
+    let compute_lemma1 (h0:heap) (vm:squash(valid_memo h0 (fixp f)))
+      : Lemma (forall x'. p x px x' ==> (let y, h1 = reify (memo_rec_extr_temp f x px x') h0 in y == fixp f x' /\ valid_memo h1 (fixp f)))
+    = forall_impl_intro (compute_lemma0 h0 vm)
+    in
+    forall_impl_intro compute_lemma1 ;
+    assert (computes #(p x px) (memo_rec_extr_temp f x px) (fixp f)) ;
+
+    memo_extr_p_computes (p x px) (memo_rec_extr_temp f x px) (fixp f) ;
+    let y, h1 = reify (memo_extr_p (p x px) (memo_rec_extr_temp f x px) x') h0 in
+    assert (y == fixp f x') ;
+    assert (valid_memo h1 (fixp f)) ;
+    assume (forall y. cont y << cont) ;
+    complete_memo_rec_extr_computes f x (cont y) h1
+and memo_rec_extr_computes :
+  (f:(x:dom -> partial_result x)) ->
+  (x:dom) ->
+  (h0:heap) ->
+  Lemma (requires (valid_memo h0 (fixp f)))
+    (ensures (let y, h1 = reify (memo_rec_extr f x) h0 in y == fixp f x /\ valid_memo h1 (fixp f)))
+    (decreases %[x ; 2 ; ()])
+= fun f x h0 ->
+  fpartial_result_lemma f x (f x) Now ;
+  complete_memo_rec_extr_computes f x (f x) h0
 
 
-(* let rec complete_memo_rec_extr_lemma *)
-(*   (f: (x:dom) -> partial_result x) *)
-(*   (x:dom) *)
-(*   (px:partial_result x) *)
-(*   (h0:heap) *)
-(*     : Lemma (requires (fpartial_result x f px /\ valid_memo_rec h0 f)) *)
-(*       (ensures (let y, h1 = reify (complete_memo_rec_extr f x px) h0 in valid_memo_rec h1 f /\ y == fixp f x)) *)
-(*       (decreases %[x ; px]) *)
-(* = *)
-(*   match px with *)
-(*   | Done _ y -> *)
-(*     assert (y == fixp f x) ; *)
-(*     assert (valid_memo_rec h0 f) *)
-(*   | Need x0 x' cont -> *)
-(*     assert (x0 == x) ; *)
-(*     let y, h0' = *)
-(*       assert (valid_memo_rec h0 f) ; *)
-(*       match reify (MEMO?.get x') h0 with *)
-(*       | Some y, h0' -> *)
-(*         valid_memo_rec_lemma f x' y h0' ; *)
-(*         assert (y == fixp f x') ; *)
-(*         y, h0' *)
-(*       | None, h0' -> *)
-(*         let px' = f x' in *)
-(*         fpartial_result_lemma f x' px' Now ; *)
-(*         assert ( %[x' ; px'] << %[x ; px]) ; *)
-(*         complete_memo_rec_extr_lemma f x' (f x') h0' ; *)
-(*         let y, h0' = reify (complete_memo_rec f x' (f x')) h0' in *)
-(*         assert (y == fixp f x') ; *)
-(*         let (), h0' = reify (MEMO?.put x' y) h0' in *)
-(*         assert (valid_memo_rec h0' f) ; *)
-(*         y,h0' *)
-(*     in *)
-(*     assert (y == fixp f x') ; *)
-(*     assert (valid_memo_rec h0' f) ; *)
-(*     assume (forall y. cont y << cont) ; *)
-(*     assert (fpartial_result x f (cont y)) ; *)
-(*     complete_memo_rec_extr_lemma f x (cont y) h0' ; *)
-(*     let y, h1 = reify (complete_memo_rec f x (cont y)) h0' in *)
-(*     let y', h1' = reify (complete_memo_rec f x px) h0 in *)
-(*     assert (y == fixp f x) ; *)
-(*     assert (valid_memo_rec h1 f) ; *)
-(*     assert ( y == y' ) ; *)
-(*     assert (y' == fixp f x) ; *)
-(*     assert ( h1 == h1' ) *)
+let memo_rec_lemma (f:(x:dom) -> partial_result x)
+ : Lemma ((memo_rec_extr f) `computes` (fixp f))
+=
+  let phi0 (h0:heap) (vm:squash(valid_memo h0 (fixp f))) (x:dom)
+    : Lemma (let y, h1 = reify (memo_rec_extr f x) h0 in y == fixp f x /\ valid_memo h1 (fixp f))
+  = give_proof vm ; memo_rec_extr_computes f x h0
+  in
+  forall_impl_intro (fun (h0:heap) (vm:squash(valid_memo h0 (fixp f))) -> forall_intro (phi0 h0 vm) <:
+    Lemma (forall x. let y, h1 = reify (memo_rec_extr f x) h0 in y == fixp f x /\ valid_memo h1 (fixp f)))
 
 
 
-(* let fix2 (f : #a:Type -> wp:(dom -> pure_wp (codom * a)) -> x0:dom -> f0:(x:dom{x << x0} -> a -> PURE (codom * a) (wp x)) -> PURE (codom * a) (wp x0)) (x0:dom) : PURE codom (fun p -> forall y. p y) *)
-(* = let wp (p:pure_post (codom * unit)) : Type0 = forall (y:codom). p (y, ()) in *)
-(*   let rec f0 (x:dom{x << x0}) () : PURE (codom * unit) wp (decreases x) = f #unit (fun _ -> wp) x f0 in *)
-(*   fst (f (fun _ -> wp) x0 f0) *)
+(* ****************************************************************************)
+(*                                                                            *)
+(*                            Example section                                 *)
+(*                                                                            *)
+(* ****************************************************************************)
 
-
-(* let memo_rec (f : #a:Type -> wp:(dom -> pure_wp (codom * a)) -> x0:dom -> f0:(x:dom{x << x0} -> a -> PURE (codom * a) (wp x)) -> PURE (codom * a) (wp x0)) (x:dom) *)
-(*   : MEMO codom (fun h0 p -> valid_memo h0 (fix f) /\ (forall h. valid_memo h (fix f) ==> p (fix f, h))) *)
-(* = *)
-(*   let rec f0 (x:dom{x << x0}) = *)
-(*     match MEMO?.get x with *)
-(*     | Some y -> *)
-(*       forall_prop_assoc_lemma2 x y (fun (x,y) -> y = (fix f)) ; *)
-(*       y *)
-(*     | None -> *)
-(*       let y = MEMO?.reflect (fun h0 -> f #heap x (reify f0) h0) in *)
 
